Redefine small step with step length

src/semantics.v
@@ -3,6 +3,11 @@ Require Import Coq.Init.Nat.
 Require Import Classes.EquivDec.
 Require Import Coq.Arith.Wf_nat.
 
+Axiom strong_induction:
+forall P : nat -> Prop,
+(forall n : nat, (forall k : nat, (k < n -> P k)) -> P n) ->
+forall n : nat, P n.
+
 Notation State := (Var -> nat).
 
 (* Semantics of expressions, which we use for both small and big-step semantics *)
@@ -26,41 +31,23 @@ Fixpoint eval_Bexp (b : Bexp) (s : State) : bool :=
   end.
 
 (* Small-step semantics *)
-Inductive small_step `{EqDec Var} : (Prog * State) -> (Prog * State) -> Prop :=
-| Sskip (s : State) : small_step (skip, s) (skip, s)
+(* We index the steps with associated costs *)
+Inductive small_step `{EqDec Var} : nat -> (Prog * State) -> (Prog * State) -> Prop :=
+| Sskip (s : State) : small_step 1 (skip, s) (skip, s)
 | Sass (s : State) (v : Var) (a : Aexp) :
-    small_step (ass v a, s) (skip, fun x => if x == v then (eval_Aexp a s) else s x)
-| SseqSkip (s1 s2 : State) (c1 c2 : Prog) (h : small_step (c1, s1) (skip, s2)) :
-    small_step (seq c1 c2, s1) (c2, s2)
-| Sseq (s1 s2 : State) (c1 c1' c2 : Prog) (h : small_step (c1, s1) (c1', s2)) (h' : c1' <> skip) :
-    small_step (seq c1 c2, s1) (seq c1' c2, s2)
+    small_step 1 (ass v a, s) (skip, fun x => if x == v then (eval_Aexp a s) else s x)
+| SseqSkip (s1 s2 : State) (c1 c2 : Prog) (n : nat) (h : small_step n (c1, s1) (skip, s2)) :
+    small_step 2 (seq c1 c2, s1) (c2, s2)
+| Sseq (s1 s2 : State) (c1 c1' c2 : Prog) (n : nat) (h : small_step n (c1, s1) (c1', s2)) (h' : c1' <> skip) :
+    small_step 1 (seq c1 c2, s1) (seq c1' c2, s2)
 | RiteT (s : State) (b : Bexp) (c1 c2 : Prog) (hb : eval_Bexp b s = true) :
-    small_step (ite b c1 c2, s) (c1, s)
+    small_step 1 (ite b c1 c2, s) (c1, s)
 | RiteF (s : State) (b : Bexp) (c1 c2 : Prog) (hb : eval_Bexp b s = false) :
-    small_step (ite b c1 c2, s) (c2, s)
+    small_step 1 (ite b c1 c2, s) (c2, s)
 | RwhileT (s : State) (b : Bexp) (c c : Prog) (hb : eval_Bexp b s = true) :
-    small_step (while b c, s) (seq c (while b c), s)
+    small_step 1 (while b c, s) (seq c (while b c), s)
 | RwhileF (s : State) (b : Bexp) (c c : Prog) (hb : eval_Bexp b s = false) :
-    small_step (while b c, s) (skip, s).
-
-
-(* We need to count skips otherwise we get weird programs like (skip ; skip) ; skip which need 0 steps
-   Maybe just do stupid case distinctions... *)
-
-Inductive small_steps `{EqDec Var} : Prog -> State -> State -> Prop :=
-| Term (s : State) : small_steps skip s s
-| Step (s1 s2 s3 : State) (c1 c2 : Prog) (h1 : small_step (c1, s1) (c2, s2))
-    (h2 : small_steps c2 s2 s3) : small_steps c1 s1 s3.
-
-Inductive counting_steps `{EqDec Var} : nat -> Prog -> State -> State -> Prop :=
-| Done (s : State) : counting_steps 0 skip s s
-| Multiple (s1 s2 s3 : State) (c1 c2 : Prog) (n : nat) (h1 : small_step (c1, s1) (c2, s2))
-    (h2 : counting_steps n c2 s2 s3) : counting_steps (1 + n) c1 s1 s3.
-
-Inductive trans `{EqDec Var} : nat -> (Prog * State) -> (Prog * State) -> Prop :=
-| One (s1 s2 : State) (c1 c2 : Prog) (h : small_step (c1, s1) (c2, s2)) : trans 1 (c1, s1) (c2, s2)
-| Trans (s1 s2 s3 : State) (c1 c2 c3 : Prog) (n : nat) (h1 : small_step (c1, s1) (c2, s2))
-    (h2 : trans n (c2, s2) (c3, s3)) : trans (1 + n) (c1, s1) (c3, s3).
+    small_step 1 (while b c, s) (skip, s).
 
 (* Big-step semantics *)
 
@@ -80,14 +67,30 @@ Inductive big_step `{EqDec Var} : Prog -> State -> State -> Prop :=
     (h1 : big_step c s1 s2) (h2 : big_step (while b c) s2 s3) : big_step (while b c) s1 s3
 | BwhileF (s : State) (b : Bexp) (c : Prog) (hb : eval_Bexp b s = false) : big_step (while b c) s s.
 
-Axiom strong_induction:
-forall P : nat -> Prop,
-(forall n : nat, (forall k : nat, (k < n -> P k)) -> P n) ->
-forall n : nat, P n.
+(* We need to count skips otherwise we get weird programs like (skip ; skip) ; skip which need 0 steps
+   Maybe just do stupid case distinctions... *)
 
+Inductive refl_trans `{EqDec Var} : nat  -> (Prog * State) -> (Prog * State) -> Prop :=
+| Refl (s : State) (c : Prog) : refl_trans 0 (c, s) (c, s)
+| Trans (s1 s2 s3 : State) (c1 c2 c3 : Prog) (n1 n2 : nat) (h1 : small_step n1 (c1, s1) (c2, s2))
+    (h2 : refl_trans n2 (c2, s2) (c3, s3)) : refl_trans (n1 + n2) (c1, s1) (c3, s3).
 
-Lemma imp_small_to_big `{EqDec Var} : forall c s1 s2, small_steps c s1 s2 -> big_step c s1 s2.
-Proof. Admitted.
+Lemma imp_small_to_big `{EqDec Var} : forall n c s1 s2, refl_trans n (c, s1) (skip, s2) -> big_step c s1 s2.
+Proof.
+  induction n; intros.
+  - inversion H0.
+    + constructor.
+    + apply PeanoNat.Nat.eq_add_0 in H2 as (H2 & H2'). rewrite H2 in h1. inversion h1.
+  - inversion H0. inversion h1.
+    + admit.
+    + admit.
+    + admit.
+    + admit.
+    + admit.
+    + admit.
+    + admit.
+    + admit.
+
 
 Lemma imp_big_to_small `{EqDec Var} : forall c s1 s2, big_step c s1 s2 -> small_steps c s1 s2.
 Proof. Admitted.
